---
title: "20181019e implicit partial differentiation"
author: "cheungngo"
date: "19 October 2018"
output: word_document
---

### Principles

For g(x,y) == constant; theorectically we can express y in terms of x, i.e. finding dy/dx  
However, most of the time it is difficult to do so  
In this case, we need to do this implicit partial differentiation:  

dy/dx = - dgdx / dgdy  

```{r,message=FALSE}
library(Ryacas)
library(mosaic)
```

##### Defined: x^2*y^3 - 6*x^3*y^2 + 2*x*y == 1

```{r}
# LHS
x = Sym('x')
y = Sym('y')
g_LHS = Solve(x^2*y^3 - 6*x^3*y^2 + 2*x*y == 1,y)
g_LHS
# OMG
```

```{r}
# RHS
g = x^2*y^3 - 6*x^3*y^2 + 2*x*y - 1
dgdx = deriv(g,x)
dgdy = deriv(g,y)
RHS = - dgdx / dgdy
PrettyForm(RHS)
```

### Extension of the theory

Suppose g(x,y,z) == c  
dz/dx = -dg/dx / dg/dz;  
dz/dy = -dg/dy / dg/dz